Merge with issue-183 #187

example/Base/SharingTests.v
@@ -8,11 +8,13 @@ From Base Require Import Free.Instance.ND.
 From Base Require Import Free.Instance.Share.
 From Base Require Import Free.Instance.Trace.
 
-From Base Require Import Free.Malias.
 From Base Require Import Free.Util.Search.
-From Base Require Import Free.Verification.Util.
+
+From Generated Require Data.List.
+From Generated Require Data.Tuple.
 
 From Base Require Import Prelude.
+Open Scope string_scope.
 
 Require Import Lists.List.
 Import List.ListNotations.
@@ -22,82 +24,104 @@ Import List.ListNotations.
 Definition evalND {A : Type} p
 := @collectVals A (run (runChoice (runNDSharing (0,0) p))).
 
-(* Shortcut to evaluate a traced program to a result and a list of logged 
+(* Shortcut to evaluate a traced program to a result and a list of logged
    messages. *)
-Definition evalTracing {A : Type} p 
+Definition evalTracing {A : Type} p
 := @collectMessages A (run (runTracing (runTraceSharing (0,0) p))).
 
-(* Shortcut to evaluate a non-deterministic partial program to a result 
+(* Shortcut to evaluate a non-deterministic partial program to a result
    list. *)
 Definition evalNDM {A : Type} p
-:= @collectVals (option A) (run (runChoice (runNDSharing (0,0) (runMaybe p)))).
+:= match (run (runMaybe (@runChoice _ _ A (runNDSharing (0,0) p)))) with
+   | Some t => Some (@collectVals A t)
+   | None => None
+   end.
 
-(* Shortcut to evaluate a traced partial program to a result and a list 
+(* Shortcut to evaluate a traced partial program to a result and a list
    of logged messages. *)
 Definition evalTraceM {A : Type} p
-:= @collectMessages (option A) 
+:= @collectMessages (option A)
    (run (runTracing (runTraceSharing (0,0) (runMaybe p)))).
 
 Section SecData.
 
   Variable Shape : Type.
   Variable Pos : Shape -> Type.
+  (* Infer Shape and Pos when tracing for convenience. *)
+  Arguments trace {_} {_} {_} {_}.
 
   Notation "'ND'" := (Injectable ND.Shape ND.Pos Shape Pos).
-  Notation "'Trace'" := (Traceable Shape Pos).
+  Notation "'Trace'" := (Injectable Trace.Shape Trace.Pos Shape Pos).
   Notation "'Maybe'" := (Injectable Maybe.Shape Maybe.Pos Shape Pos).
   Notation "'Share'" := (Injectable Share.Shape Share.Pos Shape Pos).
 
+
   (* Non-deterministic integer. *)
   Definition coin `{ND} `{I : Share} (S : Strategy Shape Pos)
-  := Choice Shape Pos (pure 0%Z) (pure 1%Z).
+  := @call Shape Pos I S _ (pure 0%Z) >>= fun c1 =>
+     @call Shape Pos I S _ (pure 1%Z) >>= fun c2 =>
+     Choice Shape Pos c1 c2.
 
   (* Non-deterministic boolean value. *)
   Definition coinB `{ND} `{I : Share} (S : Strategy Shape Pos)
-  := Choice Shape Pos (True_ Shape Pos) (False_ Shape Pos).
+  := @call Shape Pos I S _ (True_ Shape Pos) >>= fun c1 =>
+     @call Shape Pos I S _ (False_ Shape Pos) >>= fun c2 =>
+     Choice Shape Pos c1 c2.
 
   (* Non-deterministic partial integer. *)
   Definition coinM `{ND} `{Maybe} `{I : Share} (S : Strategy Shape Pos)
-  := Choice Shape Pos 
-      (@call Shape Pos I S _ (@Nothing Shape Pos _ (Integer Shape Pos)) >>= fun c0 => c0)
-      (@call Shape Pos I S _ (Just Shape Pos 1%Z) >>= fun c0 => c0).
+  := @call Shape Pos I S _ (Nothing Shape Pos) >>= fun c1 =>
+     @call Shape Pos I S _ (Just Shape Pos 1%Z) >>= fun c2 =>
+     Choice Shape Pos c1 c2.
 
   (* (0 ? 1, 2 ? 3) *)
   Definition coinPair `{ND} `{I : Share} (S : Strategy Shape Pos)
   : Free Shape Pos (Pair Shape Pos (Integer Shape Pos) (Integer Shape Pos))
-  := @call Shape Pos I S (Integer Shape Pos) 
-          (Choice Shape Pos (pure 0%Z) (pure 1%Z)) >>= fun c1 =>
-     @call Shape Pos I S (Integer Shape Pos) 
-          (Choice Shape Pos (pure 2%Z) (pure 3%Z)) >>= fun c2 =>
-     Pair_ Shape Pos c1 c2.
+  := @call Shape Pos I S _ (pure 0%Z) >>= fun c1 =>
+     @call Shape Pos I S _ (pure 1%Z) >>= fun c2 =>
+     @call Shape Pos I S (Integer Shape Pos)
+          (Choice Shape Pos c1 c2) >>= fun c3 =>
+     @call Shape Pos I S _ (pure 2%Z) >>= fun c4 =>
+     @call Shape Pos I S _ (pure 3%Z) >>= fun c5 =>
+     @call Shape Pos I S (Integer Shape Pos)
+          (Choice Shape Pos c4 c5) >>= fun c6 =>
+     Pair_ Shape Pos c3 c6.
 
   (* [0 ? 1, 2 ? 3] *)
   Definition coinList `{ND} `{I : Share} (S : Strategy Shape Pos)
   : Free Shape Pos (List Shape Pos (Integer Shape Pos))
-  := @call Shape Pos I S _ (List.Nil Shape Pos) >>= fun c1 =>
-     @call Shape Pos I S _ (Choice Shape Pos (pure 2%Z) (pure 3%Z)) >>= fun c2 =>
-     @call Shape Pos I S _ (List.Cons Shape Pos c2 c1) >>= fun c3 => 
-     @call Shape Pos I S _ (Choice Shape Pos (pure 0%Z) (pure 1%Z)) >>= fun c4 =>
-     List.Cons Shape Pos c4 c3.
-
+  := @call Shape Pos I S _ (pure 0%Z) >>= fun c1 =>
+     @call Shape Pos I S _ (pure 1%Z) >>= fun c2 =>
+     @call Shape Pos I S _ (Choice Shape Pos c1 c2) >>= fun c3 =>
+     @call Shape Pos I S _ (pure 2%Z) >>= fun c4 =>
+     @call Shape Pos I S _ (pure 3%Z) >>= fun c5 =>
+     @call Shape Pos I S _ (Choice Shape Pos c4 c5) >>= fun c6 =>
+     @call Shape Pos I S _ (List.Nil Shape Pos) >>= fun c7 =>
+     @call Shape Pos I S _ (List.Cons Shape Pos c6 c7) >>= fun c8 =>
+     List.Cons Shape Pos c3 c8.
 
   (* Traced integer. *)
-  Definition traceOne `{Trace}
-  := trace "One" (pure 1%Z).
+  Definition traceOne `{Trace} `{I : Share} (S : Strategy Shape Pos)
+  := @call Shape Pos I S _ (pure 1%Z) >>= fun c1 =>
+     trace "One" c1.
 
   (* Traced boolean values. *)
-  Definition traceTrue `{Trace}
-  := trace "True" (True_ Shape Pos).
+  Definition traceTrue `{Trace} `{I : Share} (S : Strategy Shape Pos)
+  := @call Shape Pos I S _ (True_ Shape Pos) >>= fun c1 =>
+     trace "True" c1.
 
-  Definition traceFalse `{Trace}
-  := trace "False" (False_ Shape Pos).
+  Definition traceFalse `{Trace} `{I : Share} (S : Strategy Shape Pos)
+  := @call Shape Pos I S _ (False_ Shape Pos) >>= fun c1 =>
+     trace "False" c1.
 
   (* Traced Maybe values *)
-  Definition traceNothing `{Trace} `{M : Maybe}
-  := trace "Nothing" (@Nothing Shape Pos M (Integer Shape Pos)).
+  Definition traceNothing `{Trace} `{M : Maybe} `{I : Share} (S : Strategy Shape Pos)
+  := @call Shape Pos I S _ (@Nothing Shape Pos M (Integer Shape Pos)) >>= fun c1 =>
+     trace "Nothing" c1.
 
-  Definition traceJust `{Trace} `{M : Maybe}
-  := trace "Just 1" (@Just Shape Pos M _ 1%Z).
+  Definition traceJust `{Trace} `{M : Maybe} `{I : Share} (S : Strategy Shape Pos)
+  := @call Shape Pos I S _ (@Just Shape Pos M _ 1%Z) >>= fun c1 =>
+     trace "Just 1" c1.
 
   (* (trace "0" 0, trace "1" 1) *)
   Definition tracePair `{Trace} `{I : Share} (S : Strategy Shape Pos)
@@ -111,43 +135,68 @@ Section SecData.
   (* [trace "0" 0, trace "1" 1] *)
   Definition traceList `{Trace} `{I : Share} (S : Strategy Shape Pos)
   : Free Shape Pos (List Shape Pos (Integer Shape Pos))
-  := @call Shape Pos I S _ (Nil Shape Pos) >>= fun c1 =>
-     @call Shape Pos I S _ (pure 1%Z) >>= fun c2 =>
-     @call Shape Pos I S _ (trace "1" c2) >>= fun c3 =>
-     @call Shape Pos I S _ (Cons Shape Pos c3 c1) >>= fun c4 =>
-     @call Shape Pos I S _ (pure 0%Z) >>= fun c5 =>
-     @call Shape Pos I S _ (trace "0" c5) >>= fun c6 =>
-     (Cons Shape Pos c6 c4).
+  := @call Shape Pos I S _ (pure 0%Z) >>= fun c1 =>
+     @call Shape Pos I S _ (trace "0" c1) >>= fun c2 =>
+     @call Shape Pos I S _ (pure 1%Z) >>= fun c3 =>
+     @call Shape Pos I S _ (trace "1" c3) >>= fun c4 =>
+     @call Shape Pos I S _ (Nil Shape Pos) >>= fun c5 =>
+     @call Shape Pos I S _ (Cons Shape Pos c4 c5) >>= fun c6 =>
+     (Cons Shape Pos c2 c6).
+
+  (* [trace "1" 1, trace "2" 2, trace "3" 3] *)
+  Definition traceList3 `{Trace} `{I : Share} (S : Strategy Shape Pos)
+  : Free Shape Pos (List Shape Pos (Integer Shape Pos))
+  := @call Shape Pos I S _ (pure 1%Z) >>= fun c1 =>
+     @call Shape Pos I S _ (trace "1" c1) >>= fun c2 =>
+     @call Shape Pos I S _ (pure 2%Z) >>= fun c3 =>
+     @call Shape Pos I S _ (trace "2" c3) >>= fun c4 =>
+     @call Shape Pos I S _ (pure 3%Z) >>= fun c5 =>
+     @call Shape Pos I S _ (trace "3" c5) >>= fun c6 =>
+     @call Shape Pos I S _ (Nil Shape Pos) >>= fun c7 =>
+     @call Shape Pos I S _ (Cons Shape Pos c6 c7) >>= fun c8 =>
+     @call Shape Pos I S _ (Cons Shape Pos c4 c8) >>= fun c9 =>
+     (Cons Shape Pos c2 c9).
+
+
 
 End SecData.
 
 (* Arguments sentences for the data. *)
-Arguments coin {_} {_} {_} {_} _.
-Arguments coinB {_} {_} {_} {_} _.
-Arguments coinM {_} {_} {_} {_} {_} _.
-Arguments coinPair {_} {_} {_} {_} _.
-Arguments coinList {_} {_} {_} {_} _.
+Arguments coin {_} {_} {_} {_}.
+Arguments coinB {_} {_} {_} {_}.
+Arguments coinM {_} {_} {_} {_} {_}.
+Arguments coinPair {_} {_} {_} {_}.
+Arguments coinList {_} {_} {_} {_}.
 Arguments traceOne {_} {_} {_}.
 Arguments traceTrue {_} {_} {_}.
 Arguments traceFalse {_} {_} {_}.
 Arguments traceNothing {_} {_} {_} {_}.
 Arguments traceJust {_} {_} {_} {_}.
-Arguments tracePair {_} {_} {_} {_} _.
-Arguments traceList {_} {_} {_} {_} _.
-
+Arguments tracePair {_} {_} {_}.
+Arguments traceList {_} {_} {_}.
+Arguments traceOne {_} {_} {_} {_}.
+Arguments traceTrue {_} {_} {_} {_}.
+Arguments traceFalse {_} {_} {_} {_}.
+Arguments traceNothing {_} {_} {_} {_} {_}.
+Arguments traceJust {_} {_} {_} {_} {_}.
+Arguments tracePair {_} {_} {_} {_}.
+Arguments traceList {_} {_} {_} {_}.
+Arguments traceList3 {_} {_} {_} {_}.
 (* Test functions *)
+
 Section SecFunctions.
 
-  Set Implicit Arguments.
+  (*Set Implicit Arguments.*)
   Variable Shape : Type.
   Variable Pos : Shape -> Type.
   Variable A : Type.
+
   Notation "'FreeA'" := (Free Shape Pos A).
   Notation "'ShareArgs'" := (ShareableArgs Shape Pos A).
   Notation "'Share'" := (Injectable Share.Shape Share.Pos Shape Pos).
   Notation "'Maybe'" := (Injectable Maybe.Shape Maybe.Pos Shape Pos).
 
-  (* Simple sharing: 
+  (* Simple sharing:
      let sx = fx in f sx sx *)
   Definition doubleShared `{I : Share} `{SA : ShareArgs} (S : Strategy Shape Pos)
                         (f : FreeA -> FreeA -> FreeA)
@@ -156,18 +205,18 @@ Section SecFunctions.
   := @share Shape Pos I S A SA fx >>= fun sx => f sx sx.
 
   (* Nested sharing:
-     let sx = fx 
+     let sx = fx
          sy = f sx sx
      in f sy sy *)
   Definition doubleSharedNested `{I : Share} `{SA : ShareArgs} (S : Strategy Shape Pos)
                                 (f : FreeA -> FreeA -> FreeA)
                                 (fx : FreeA)
    : FreeA
-  := @share Shape Pos I S A SA fx >>= fun sx => 
+  := @share Shape Pos I S A SA fx >>= fun sx =>
      @share Shape Pos I S A SA (f sx sx) >>= fun sy =>
     f sy sy.
 
-  (* let sx = fx  
+  (* let sx = fx
          sy = f sx sx
          sz = fy
     in f sy sz *)
@@ -177,7 +226,7 @@ Section SecFunctions.
   : FreeA
   := @share Shape Pos I S A SA fx >>= fun sx =>
      @call Shape Pos I S A (f sx sx) >>= fun sy =>
-     @call Shape Pos I S A fy >>= fun sz => 
+     @call Shape Pos I S A fy >>= fun sz =>
      f sy sz.
 
   (*
@@ -202,7 +251,7 @@ Section SecFunctions.
 
   (* Deep sharing. *)
 
-  (* 
+  (*
   let sx = fx
       c1 = fst sx
       c2 = fst sx
@@ -212,12 +261,12 @@ Section SecFunctions.
                         (f : FreeA -> FreeA -> FreeA)
                         (fx : Free Shape Pos (Pair Shape Pos A A))
    : FreeA
-  := @share Shape Pos I S (Pair Shape Pos A A) _ fx >>= fun sx => 
-     @call Shape Pos I S A (fstPair Shape Pos sx) >>= fun c1 =>
-     @call Shape Pos I S A (fstPair Shape Pos sx) >>= fun c2 =>
+  := @share Shape Pos I S (Pair Shape Pos A A) _ fx >>= fun sx =>
+     @call Shape Pos I S A (Tuple.fst Shape Pos sx) >>= fun c1 =>
+     @call Shape Pos I S A (Tuple.fst Shape Pos sx) >>= fun c2 =>
       f c1 c2.
 
-  (* 
+  (*
   let sx = fl in head sx + head sx
   Flattened version:
   let sx = fl
@@ -230,11 +279,51 @@ Section SecFunctions.
                         (fl : Free Shape Pos (List Shape Pos A))
    : FreeA
   := @share Shape Pos I S (List Shape Pos A) _ fl >>= fun sx =>
-     @call Shape Pos I S A (headList Shape Pos P sx) >>= fun c1 =>
-     @call Shape Pos I S A (headList Shape Pos P sx) >>= fun c2 =>
+     @call Shape Pos I S A (List.head Shape Pos P sx) >>= fun c1 =>
+     @call Shape Pos I S A (List.head Shape Pos P sx) >>= fun c2 =>
               f c1 c2.
 
+(* Recursive functions *)
+
+
+  (*
+   tails :: [a] -> [[a]]
+   tails xs = xs : case xs of
+   []      -> []
+   x : xs' -> tails xs'
+  *)
+  (* fxs' can not be shared because the termination checker does not accept that definition
+     as well-formed. But since xs0 is shared (in tails), its component fxs' is also automatically shared. *)
+  Fixpoint tails_0
+     `{Share}
+     (S : Strategy Shape Pos)
+     (xs0 : List Shape Pos A) {struct xs0}
+   : Free Shape Pos (List Shape Pos (List Shape Pos A))
+    := match xs0 with
+       | List.nil          =>  Nil Shape Pos
+       | List.cons _ fxs' =>  @call Shape Pos _ S _ (fxs' >>= fun xs'0 => tails_0 S xs'0) >>= fun c1 =>
+                              Cons Shape Pos fxs' c1
+       end.
+
+  Definition tails
+    `{Share}
+    `{ShareArgs}
+    (S : Strategy Shape Pos)
+    (fxs : Free Shape Pos (List Shape Pos A))
+    : Free Shape Pos (List Shape Pos (List Shape Pos A))
+   := @share Shape Pos _ S _ _ fxs >>= fun fxs0 =>
+      @call Shape Pos _ S _ (fxs0 >>= fun xs0 => tails_0 S xs0) >>= fun c1 =>
+        Cons Shape Pos fxs0 c1.
+
 End SecFunctions.
+
+Arguments doubleShared {_} {_} {_} {_} {_}.
+Arguments doubleSharedClash {_} {_} {_} {_} {_}.
+Arguments doubleSharedNested {_} {_} {_} {_} {_}.
+Arguments doubleSharedRec {_} {_} {_} {_} {_}.
+Arguments doubleDeepSharedPair {_} {_} {_} {_} {_}.
+Arguments doubleDeepSharedList {_} {_} {_} {_} {_}.
+Arguments tails {_} {_} {_} {_} {_}.
 
 (* Some notations for convenience.
    Since we only provide the sharing instance and functions when the handlers
@@ -245,10 +334,10 @@ Notation "'Cbv_'" := (Cbv _ _).
 Notation "'addInteger_'" := (addInteger _ _).
 Notation "'orBool_'" := (orBool _ _).
 
-
 (* ---------------------- Test cases without sharing ----------------------- *)
 
-(* 
+
+(*
 0?1 + 0?1
 = 0+0 ? 0+1 ? 1+0 ? 1+1
 = 0 ? 1 ? 1 ? 2
@@ -261,9 +350,9 @@ Proof. constructor. Qed.
 trace "One" 1 + trace "One" 1
 => The message should be logged twice and the result should be 2.
 *)
-Example exAddNoSharingTrace 
-: evalTracing (nf (doubleShared Cbn_ addInteger_ traceOne))
-  = (2%Z,["One"%string;"One"%string]).
+Example exAddNoSharingTrace
+: evalTracing (nf (doubleShared Cbn_ addInteger_ (traceOne Cbn_)))
+  = (2%Z,["One";"One"]).
 Proof. constructor. Qed.
 
 (*
@@ -272,18 +361,18 @@ Proof. constructor. Qed.
 = true ? (true ? false)
 = true ? true ? false
 *)
-Example exOrNDNoSharing 
+Example exOrNDNoSharing
  : evalND (nf (doubleShared Cbn_ orBool_ (coinB Cbn_))) = [true;true;false].
 Proof. constructor. Qed.
 
 (*
 (trace "True" true) or (trace "True" true)
-=> The second argument is not evaluated, so the result should be true and the 
+=> The second argument is not evaluated, so the result should be true and the
    message should be logged only once.
 *)
-Example exOrTrueTracingNoSharing 
- : evalTracing (nf (doubleShared Cbn_ orBool_ traceTrue))
-   = (true,["True"%string]).
+Example exOrTrueTracingNoSharing
+ : evalTracing (nf (doubleShared Cbn_ orBool_ (traceTrue Cbn_)))
+   = (true,["True"]).
 Proof. constructor. Qed.
 
 (*
@@ -291,9 +380,9 @@ Proof. constructor. Qed.
 => Both arguments are evaluated, so the result should be false and the message
    should be logged twice.
 *)
-Example exOrFalseTracingNoSharing 
- : evalTracing (nf (doubleShared Cbn_ orBool_ traceFalse))
-   = (false,["False"%string;"False"%string]).
+Example exOrFalseTracingNoSharing
+ : evalTracing (nf (doubleShared Cbn_ orBool_ (traceFalse Cbn_)))
+   = (false,["False";"False"]).
 Proof. constructor. Qed.
 
 (*
@@ -302,47 +391,44 @@ Proof. constructor. Qed.
    should be logged.
 *)
 Example exOrMixedTracingNoSharing
- : evalTracing (nf (orBool_ traceFalse traceTrue))
-   = (true,["False"%string;"True"%string]).
+ : evalTracing (nf (orBool_ (traceFalse Cbn_) (traceTrue Cbn_)))
+   = (true,["False";"True"]).
 Proof. constructor. Qed.
 
 (*
 (Nothing ? Just 1) + (Nothing ? Just 1)
-= (Nothing + (Nothing ? Just 1)) ? (Just 1 + (Nothing ? Just 1))
-= Nothing ? (Just 1 + (Nothing ? Just 1))
-= Nothing ? (Just 1 + Nothing ? Just 1 + Just 1)
-= Nothing ? Nothing ? Just 2
+= Nothing
 *)
 Example exNDMNoSharing
- : evalNDM (nf (doubleShared Cbn_ addInteger_ (coinM Cbn_))) = [None;None;Some 2%Z].
+ : evalNDM (nf (doubleShared Cbn_ addInteger_ (coinM Cbn_))) = None.
 Proof. constructor. Qed.
 
-(* 
+(*
 trace "Nothing" Nothing + trace "Nothing" Nothing
 => The second argument is not evaluated due to >>=, so the message should
    only be logged once and the result should be Nothing (i.e. None in Coq).
 *)
 Example exTraceNothingNoSharing
- : evalTraceM (nf (doubleShared Cbn_ addInteger_ traceNothing))
-   = (None,["Nothing"%string]).
+ : evalTraceM (nf (doubleShared Cbn_ addInteger_ (traceNothing Cbn_)))
+   = (None,["Nothing"]).
 Proof. constructor. Qed.
 
 (*
 trace "Just 1" (Just 1) + trace "Just 1" (Just 1)
-=> Since there is no sharing, the message should be logged twice and the 
+=> Since there is no sharing, the message should be logged twice and the
    result should be Just 2 (Some 2 in Coq).
 *)
 Example exTraceJustNoSharing
- : evalTraceM (nf (doubleShared Cbn_ addInteger_ traceJust))
-   = (Some 2%Z,["Just 1"%string;"Just 1"%string]).
+ : evalTraceM (nf (doubleShared Cbn_ addInteger_ (traceJust Cbn_)))
+   = (Some 2%Z,["Just 1";"Just 1"]).
 Proof. constructor. Qed.
 
 
 (* --------------------- Test cases for simple sharing --------------------- *)
 
 (*
-let sx = 0 ? 1 
-in sx + sx 
+let sx = 0 ? 1
+in sx + sx
 = 0+0 ? 1+1
 = 0 ? 2
 *)
@@ -353,7 +439,7 @@ Proof. constructor. Qed.
 
 (* Strict evaluation also leads to consistent choices. *)
 Example exAddSharingNDStrict : evalND (nf (doubleShared Cbv_
-  addInteger_ (coin Cbv_))) 
+  addInteger_ (coin Cbv_)))
   = [0%Z;2%Z].
 Proof. constructor. Qed.
 
@@ -362,15 +448,15 @@ let sx = trace "One" 1
 in sx + sx
 => The message should be logged once and the result should be 2.
 *)
-Example exAddSharingTrace 
- : evalTracing (nf (doubleShared Cbneed_ addInteger_ traceOne))
- = (2%Z,["One"%string]).
+Example exAddSharingTrace
+ : evalTracing (nf (doubleShared Cbneed_ addInteger_ (traceOne Cbneed_)))
+ = (2%Z,["One"]).
 Proof. constructor. Qed.
 
 (* Strict evaluation also leads to the message being logged only once. *)
 Example exAddSharingTraceStrict
- : evalTracing (nf (doubleShared Cbv_ addInteger_ traceOne))
- = (2%Z,["One"%string]).
+ : evalTracing (nf (doubleShared Cbv_ addInteger_ (traceOne Cbv_)))
+ = (2%Z,["One"]).
 Proof. constructor. Qed.
 
 (*
@@ -390,19 +476,19 @@ Proof. constructor. Qed.
 
 (*
 let sx = trace "True" true
-in sx or sx 
+in sx or sx
 => The second argument is not evaluated, so sharing makes no difference here.
    The message should be logged once and the result should be true.
 *)
 Example exOrTrueTraceSharing
- : evalTracing (nf (doubleShared Cbneed_ orBool_ traceTrue))
-   = (true,["True"%string]).
+ : evalTracing (nf (doubleShared Cbneed_ orBool_ (traceTrue Cbneed_)))
+   = (true,["True"]).
 Proof. constructor. Qed.
 
 (* Strict evaluation also leads to the message being logged only once. *)
 Example exOrTrueTraceSharingStrict
- : evalTracing (nf (doubleShared Cbv_ orBool_ traceTrue))
-   = (true,["True"%string]).
+ : evalTracing (nf (doubleShared Cbv_ orBool_ (traceTrue Cbv_)))
+   = (true,["True"]).
 Proof. constructor. Qed.
 
 (*
@@ -412,19 +498,18 @@ in sx or sx
 only be logged once and the result should be false.
 *)
 Example exOrFalseTraceSharing
- : evalTracing (nf (doubleShared Cbneed_ orBool_ traceFalse))
-   = (false,["False"%string]).
+ : evalTracing (nf (doubleShared Cbneed_ orBool_ (traceFalse Cbneed_)))
+   = (false,["False"]).
 Proof. constructor. Qed.
 
 (*
 let sx = Nothing ? Just 1
 in sx + sx
-= Nothing + Nothing ? Just 1 + Just 1
-= Nothing ? Just 2
+= Nothing
 *)
 Example exNDMSharing
  : evalNDM (nf (doubleShared Cbneed_ addInteger_ (coinM Cbneed_)))
-   = [None;Some 2%Z].
+   = None.
 Proof. constructor. Qed.
 
 (*
@@ -434,45 +519,45 @@ in sx + sx
    due to >>=.
 *)
 Example exTraceNothingSharing
- : evalTraceM (nf (doubleShared Cbneed_ addInteger_ traceNothing))
-   = (None,["Nothing"%string]).
+ : evalTraceM (nf (doubleShared Cbneed_ addInteger_ (traceNothing Cbneed_)))
+   = (None,["Nothing"]).
 Proof. constructor. Qed.
 
 (*
 let sx = trace "Just 1" (Just 1)
-in sx + sx 
-=> The message should only be logged once due to sharing and the result 
+in sx + sx
+=> The message should only be logged once due to sharing and the result
    should be Some 2.
 *)
 Example exTraceJustSharing
- : evalTraceM (nf (doubleShared Cbneed_ addInteger_ traceJust))
-   = (Some 2%Z,["Just 1"%string]).
+ : evalTraceM (nf (doubleShared Cbneed_ addInteger_ (traceJust Cbneed_)))
+   = (Some 2%Z,["Just 1"]).
 Proof. constructor. Qed.
 
 (* --------------------- Test cases for nested sharing --------------------- *)
 
-(* 
-let sx = 0 ? 1 
-    sy = sx + sx 
-in sy + sy 
-= (0+0)+(0+0) ? (1+1)+(1+1) 
-= 0 ? 4 
+(*
+let sx = 0 ? 1
+    sy = sx + sx
+in sy + sy
+= (0+0)+(0+0) ? (1+1)+(1+1)
+= 0 ? 4
 *)
 Example exAddNestedSharingND : evalND (nf (doubleSharedNested Cbneed_
-                                                          addInteger_ 
+                                                          addInteger_
                                                           (coin Cbneed_)))
                                = [0%Z;4%Z].
 Proof. constructor. Qed.
 
-(* 
+(*
 let sx = trace "One" 1
-    sy = sx + sx 
-in sy + sy 
-=> The message should only be logged once and the result should be 4. 
+    sy = sx + sx
+in sy + sy
+=> The message should only be logged once and the result should be 4.
 *)
-Example exAddNestedSharingTrace 
- : evalTracing (nf (doubleSharedNested Cbneed_ addInteger_ traceOne))
-   = (4%Z,["One"%string]).
+Example exAddNestedSharingTrace
+ : evalTracing (nf (doubleSharedNested Cbneed_ addInteger_ (traceOne Cbneed_)))
+   = (4%Z,["One"]).
 Proof. constructor. Qed.
 
 (*
@@ -493,9 +578,9 @@ in sy or sy
 => The message should only be logged once due to non-strictness
    and the result should be true.
 *)
-Example exOrNestedTrueTracing 
- : evalTracing (nf (doubleSharedNested Cbneed_ orBool_ traceTrue))
-   = (true,["True"%string]).
+Example exOrNestedTrueTracing
+ : evalTracing (nf (doubleSharedNested Cbneed_ orBool_ (traceTrue Cbneed_)))
+   = (true,["True"]).
 Proof. constructor. Qed.
 
 (*
@@ -506,11 +591,11 @@ in sy or sy
    and the result should be false.
 *)
 Example exOrNestedFalseTracing
- : evalTracing (nf (doubleSharedNested Cbneed_ orBool_ traceFalse))
-   = (false, ["False"%string]).
+ : evalTracing (nf (doubleSharedNested Cbneed_ orBool_ (traceFalse Cbneed_)))
+   = (false, ["False"]).
 Proof. constructor. Qed.
 
-(* 
+(*
 let sx = 0 ? 1
     sy = sx + sx
     sz = 0 ? 1
@@ -534,8 +619,8 @@ in sy + sz
 *)
 Example exAddClashSharingTracing
  : evalTracing (nf (doubleSharedClash Cbneed_ addInteger_
-                                  traceOne traceOne))
-   = (3%Z,["One"%string;"One"%string]).
+                                  (traceOne Cbneed_) (traceOne Cbneed_)))
+   = (3%Z,["One";"One"]).
 Proof. constructor. Qed.
 
 (*
@@ -557,13 +642,13 @@ let sx = trace "True" true
     sy = sx or sx
     sz = trace "True" true
 in sy or sz
-=> The message should only be logged once due to non-strictness and the 
+=> The message should only be logged once due to non-strictness and the
    result should be true.
 *)
 Example exOrClashTrueTracing
  : evalTracing (nf (doubleSharedClash Cbneed_ orBool_
-                                  traceTrue traceTrue))
-   = (true,["True"%string]).
+                                  (traceTrue Cbneed_) (traceTrue Cbneed_)))
+   = (true,["True"]).
 Proof. constructor. Qed.
 
 (*
@@ -577,8 +662,8 @@ in sy or sz
 *)
 Example exOrClashFalseTracing
  : evalTracing (nf (doubleSharedClash Cbneed_ orBool_
-                                  traceFalse traceFalse))
-   = (false,["False"%string;"False"%string]).
+                                  (traceFalse Cbneed_) (traceFalse Cbneed_)))
+   = (false,["False";"False"]).
 Proof. constructor. Qed.
 
 (*
@@ -604,15 +689,15 @@ let sx = 1
     sy = sx + trace "One" 1
     sz = sy + trace "One" 1
 in sx + (sy + (sz + 1))
-=> The message should be logged once for sy and once for sz, so it should be 
-   logged twice in total. 
-   sx has the value 1, sy has the value 2 and sz has the value 3, so the 
+=> The message should be logged once for sy and once for sz, so it should be
+   logged twice in total.
+   sx has the value 1, sy has the value 2 and sz has the value 3, so the
    final value should be 1 + 2 + 3 + 1 = 7.
 *)
 Example exAddRecSharingTracing
  : evalTracing (nf (doubleSharedRec Cbneed_ addInteger_
-                                traceOne traceOne 1%Z))
-   = (7%Z,["One"%string;"One"%string]).
+                                (traceOne Cbneed_) (traceOne Cbneed_) 1%Z))
+   = (7%Z,["One";"One"]).
 Proof. constructor. Qed.
 
 (*
@@ -636,9 +721,9 @@ in sx or (sy or (sz or false))
   false or ((false or false) or ((false or (true ? false)) or false))
 = (false or true) or ((true or (true ? false)) or false) ?
   (false or false) or ((false or (true ? false)) or false)
-= true ? 
+= true ?
   (false or (true ? false)) or false
-= true ? 
+= true ?
   (true ? false) or false
 = true ?
   true or false ?
@@ -650,18 +735,18 @@ Example exOrRecSharingNDFalse
    = [true;true;false].
 Proof. constructor. Qed.
 
-(* 
+(*
 let sx = false
     sy = sx or (trace "True" true)
     sz = sy or (trace "True" true)
 in sx or (sy or (sz or false))
-=> sy has the value true, so sz is not evaluated. The message should only 
+=> sy has the value true, so sz is not evaluated. The message should only
    be logged once and the result should be true.
 *)
 Example exOrRecTrueTracing
  : evalTracing (nf (doubleSharedRec Cbneed_ orBool_
-                                traceTrue traceTrue false))
-   = (true,["True"%string]).
+                                (traceTrue Cbneed_) (traceTrue Cbneed_) false))
+   = (true,["True"]).
 Proof. constructor. Qed.
 
 (*
@@ -675,8 +760,8 @@ in sx or (sy or (sz or false))
 *)
 Example exOrRecFalseTracing
  : evalTracing (nf (doubleSharedRec Cbneed_ orBool_
-                                traceFalse traceFalse false))
-   = (false,["False"%string;"False"%string]).
+                                (traceFalse Cbneed_) (traceFalse Cbneed_) false))
+   = (false,["False";"False"]).
 Proof. constructor. Qed.
 
 
@@ -689,7 +774,7 @@ in fst sx + fst sx
 = (0 + 0) ? (1 + 1)
 = 0 ? 2
 *)
-Example exAddDeepPairND 
+Example exAddDeepPairND
  : evalND (nf (doubleDeepSharedPair Cbneed_ addInteger_ (coinPair Cbneed_)))
   = [0%Z;2%Z].
 Proof. constructor. Qed.
@@ -700,36 +785,110 @@ in head sx + head sx
 = 0 ? 2
 *)
 Example exAddDeepListND
- : evalND (nf 
-  (doubleDeepSharedList (ND.Partial _ _) 
+ : evalND (nf
+  (doubleDeepSharedList (ND.Partial _ _)
    Cbneed_ addInteger_ (coinList Cbneed_)))
  = [0%Z;2%Z].
 Proof. constructor. Qed.
 
-(* 
+(*
 let sx = (trace "0" 0, trace "1" 1)
-in fst sx + fst sx 
-=> The pair is shared, so the effects inside the pair should be shared as 
-   well. Since we take the first element twice, the second tracing message ("1") 
-   should not be logged and the first should be shared and thus logged once. 
+in fst sx + fst sx
+=> The pair is shared, so the effects inside the pair should be shared as
+   well. Since we take the first element twice, the second tracing message ("1")
+   should not be logged and the first should be shared and thus logged once.
 *)
 Example exAddDeepPairTrace
  : evalTracing (nf (doubleDeepSharedPair Cbneed_ addInteger_ (tracePair Cbneed_)))
-  = (0%Z, ["0"%string]).
+  = (0%Z, ["0"]).
 Proof. constructor. Qed.
 
-(* 
+(*
 let sx = (trace "0" 0, trace "1" 1)
-in head sx + head sx 
-=> The list is shared, so the effects inside the pair should be shared as 
-   well. Since we take the first element twice, the second tracing message ("1") 
+in head sx + head sx
+=> The list is shared, so the effects inside the pair should be shared as
+   well. Since we take the first element twice, the second tracing message ("1")
    should not be logged and the first should be shared and thus logged once.
    Because head is partial and we use the Maybe instance of Partial, the result
    should be Some 0 instead of simply 0.
 *)
 Example exAddDeepListTrace
- : evalTraceM (nf 
+ : evalTraceM (nf
    (doubleDeepSharedList (Maybe.Partial _ _)
     Cbneed_ addInteger_ (traceList Cbneed_)))
-  = (Some 0%Z, ["0"%string]).
+  = (Some 0%Z, ["0"]).
 Proof. constructor. Qed.
+
+(*
+  sumTails :: [Integer] -> Integer
+  sumTails l = sum (map sum (tails l))
+*)
+Definition sumTails
+  (Shape : Type) (Pos : Shape -> Type)
+  `{I : Injectable Share.Shape Share.Pos Shape Pos}
+  (S : Strategy Shape Pos)
+  (l : Free Shape Pos (List Shape Pos (Integer Shape Pos)))
+  : Free Shape Pos (Integer Shape Pos)
+ := List.sum Shape Pos
+      (List.map Shape Pos (pure (fun fxs => List.sum Shape Pos fxs))
+                     (tails S l)).
+
+(* Evaluation of sumTails [trace "1" 1, trace "2" 2, trace "3" 3] *)
+(* = sum (map (sum [trace "1" 1, trace "2" 2, trace "3" 3] : [trace "2" 2, trace "3" 3] : [trace "3" 3] : [])) *)
+
+(* Call-by-need *)
+(* Due to sharing, each number should be logged only once. *)
+Example exSumTailsTracingCbneed : evalTracing (nf (sumTails _ _ Cbneed_ (traceList3 Cbneed_)))
+ = (14%Z,["1";"2";"3"]).
+Proof. constructor. Qed.
+
+(* Call-by-name *)
+(* Each time an element is evaluated, its message is logged again.
+   Only one of the lists in the result of tails contains 1, two contain 2,
+   and three contain 3. Therefore, "1" should be logged once, "2" twice and
+   "3" three times. *)
+Example exSumTailsTracingCbn : evalTracing (nf (sumTails _ _ Cbn_ (traceList3 Cbn_)))
+ = (14%Z,["1";"2";"3";"2";"3";"3"]).
+Proof. constructor. Qed.
+
+(* Call-by-value *)
+(* The tracing effect is evaluated immediately, so we should only log each number once. *)
+Example exSumTailsTracingCbv : evalTracing (nf (sumTails _ _ Cbv_ (traceList3 Cbv_)))
+ = (14%Z,["1";"2";"3"]).
+Proof. constructor. Qed.
+
+(* Evaluation of sumTails [0 ? 1, 2 ? 3] *)
+
+(* Call-by-need *)
+(* sumTails [0 ? 1, 2 ? 3]
+  = sum (map sum (tails [0 ? 1, 2 ? 3]))
+  = sum (map sum ( [0 ? 1, 2 ? 3] : tails [ 2 ? 3 ]  ))
+  = sum (map sum ( [0 ? 1, 2 ? 3] : ([2 ? 3] : [])  ))
+  = sum (map sum ([[0,2],[2]] ? [[0,3], [3]] ? [[1,2],[2]] ? [[1,3],[3]] ))
+  = sum ([2,2] ? [3,3] ? [3,2] ? [4,3])
+  = 4 ? 6 ? 5 ? 7
+*)
+Example exSumTailsNDCbneed : evalND (nf (sumTails _ _ Cbneed_ (coinList Cbneed_)))
+ = [4%Z;6%Z;5%Z;7%Z].
+Proof. constructor. Qed.
+
+(* Call-by-name *)
+(*
+  sumTails [0 ? 1, 2 ? 3]
+  = sum (map sum (tails [0 ? 1, 2 ? 3]))
+  = sum (map sum ( [0 ? 1, 2 ? 3] : tails [ 2 ? 3 ]  ))
+  = sum (map sum ( [0 ? 1, 2 ? 3] : ([2 ? 3] : [])  ))
+  = sum ([2,2] ? [3,2] ? [2,3] ? [3,3] ? [3,2] ? [3,3] ? [4,2] ? [4,3])
+  = 4 ? 5 ? 5 ? 6 ? 5 ? 6 ? 6 ? 7
+*)
+Example exSumTailsNDCbn : evalND (nf (sumTails _ _ Cbn_ (coinList Cbn_)))
+ = [4%Z;5%Z;5%Z;6%Z;5%Z;6%Z;6%Z;7%Z].
+Proof. constructor. Qed.
+
+(* Call-by-value *)
+(* Because the non-determinism is evaluated immediately, the result should be
+   the same as with call-by-need evaluation. *)
+Example exSumTailsNDCbv : evalND (nf (sumTails _ _ Cbv_ (coinList Cbv_)))
+ = [4%Z;6%Z;5%Z;7%Z].
+Proof. constructor. Qed.
+
